Games/gameLib_fix/Zermelo.lean
@@ -1,0 +1,31 @@
+
+import Games.gameLib_fix.Termination
+
+
+lemma Game_World.not_has_WL (g : Game_World α β) (h : ¬ g.has_WL) :
+  ¬ g.is_fst_win ∧ ¬ g.is_snd_win :=
+  by
+  contrapose h
+  simp_rw [not_and_or, not_not] at h
+  rw [not_not]
+  cases' h with h h
+  · exact Game_World.has_WL.wf h
+  ·  exact Game_World.has_WL.ws h
+
+
+inductive History_good : (α) → (α → List β → (β → Prop)) → (α → List β → (β → Prop)) → (List β) → (β) → Prop where
+| mk (ini : α) (f_law s_law : α → List β → (β → Prop)) (hist : List β) (act : β) (leg : Hist_legal ini f_law s_law (act :: hist)) (good : ∃ next : β, History_good ini f_law s_law (act :: hist) next) : History_good ini f_law s_law hist act
+  -- neutral : (State_of_hist act :: hist).neutral
+
+--set_option trace.Elab.inductive true in
+--set_option trace.Kernel true in
+inductive test : Option Nat → Nat → Prop where
+| mk (k) (n) (h : ∃ m, 1 = 0 →  test (k+1) m) : test (k) n
+
+lemma Game_World.Zermelo (g : Game_World α β) :
+  g.isWL → g.has_WL :=
+  by
+  intro h
+  contrapose h
+  unfold Game_World.isWL
+  push_neg
